dafny/abstract-interpreter/AbstractInterpretation.dfy
@@ -1,6 +1,6 @@
 module AbstractInterpretation {
 
-    datatype CFG<InstructionType> = Node(nodes: seq<InstructionType>, edges: nat -> seq<nat>)
+    datatype CFG<InstructionType> = CFG(nodes: seq<InstructionType>, edges: nat -> seq<nat>)
 
     opaque function join<T>(state1: T, state2: T) : T 
     {
